Organized FMap structures and some files

src/Semantics.v
@@ -1,1088 +1,445 @@
-Require Import Bool List String Structures.Equalities.
-Require Import Lib.Struct Lib.Word Lib.CommonTactics Lib.StringBound Lib.ilist Lib.FMap Syntax.
-Require Import FunctionalExtensionality Program.Equality Eqdep Eqdep_dec.
+Require Import Lib.CommonTactics Lib.FMap Lib.Struct.
+Require Export Syntax SemanticsExprAction. (* Should be "Require Export" *)
+Require Import String List.
 
 Set Implicit Arguments.
 
-(* TODO: may move to lib/Struct.v *)
-Lemma opt_some_eq: forall {A} (v1 v2: A), Some v1 = Some v2 -> v1 = v2.
-Proof. intros; inv H; reflexivity. Qed.
+Record LabelTP {A : Type} :=
+  { ruleMeth : option A
+  ; dms : CallsT
+  ; cms : CallsT
+  }.
 
-Lemma typed_type_eq:
-  forall {A} (a1 a2: A) (B: A -> Type) (v1: B a1) (v2: B a2),
-    {| objType := a1; objVal := v1 |} = {| objType := a2; objVal := v2 |} ->
-    exists (Heq: a1 = a2), match Heq with eq_refl => v1 end = v2.
-Proof. intros; inv H; exists eq_refl; reflexivity. Qed.
+Arguments LabelTP : clear implicits.
 
-Lemma typed_eq:
-  forall {A} (a: A) (B: A -> Type) (v1 v2: B a),
-    {| objType := a; objVal := v1 |} = {| objType := a; objVal := v2 |} ->
-    v1 = v2.
-Proof. intros; inv H; apply Eqdep.EqdepTheory.inj_pair2 in H1; assumption. Qed.
+Definition LabelT := LabelTP True.
+Definition RuleLabelT := LabelTP string.
 
-(* concrete representations of data kinds *)
-Fixpoint type (t: Kind): Type :=
-  match t with
-    | Bool => bool
-    | Bit n => word n
-    | Vector nt n => word n -> type nt
-    | Struct attrs => forall i, @GetAttrType _ (map (mapAttr type) attrs) i
+Definition mapLabelTP {A B : Type} (f : A -> B) (l : LabelTP A)
+: LabelTP B :=
+  match l with
+    | Build_LabelTP rm dms cms => Build_LabelTP (option_map f rm) dms cms
   end.
 
-(*
-Fixpoint fullType (k : FullKind) : Type := match k with
-  | SyntaxKind t => type t
-  | NativeKind t => t
+Definition NotBothRule (rm1 rm2 : option string) : Prop :=
+  rm1 = None \/ rm2 = None.
+
+Definition CanCombine (ul1 ul2: RegsT * RuleLabelT) : Prop :=
+  M.Disj (fst ul1) (fst ul2) /\
+  NotBothRule (ruleMeth (snd ul1)) (ruleMeth (snd ul2)) /\
+  M.Disj (dms (snd ul1)) (dms (snd ul2)) /\
+  M.Disj (cms (snd ul1)) (cms (snd ul2)).
+
+Definition mergeLabel {A : Type} (l1 l2 : LabelTP A) : LabelTP A := 
+  match l1, l2 with
+      Build_LabelTP rm1 ds1 cs1, Build_LabelTP rm2 ds2 cs2 =>
+      Build_LabelTP (match rm1 with | Some r => Some r | None => rm2 end) 
+                    (M.union ds1 ds2) 
+                    (M.union cs1 cs2)
   end.
- *)
 
-Section WordFunc.
+Definition equivalent {A : Type} (l1 l2 : LabelTP A)
+           (p : LabelTP A -> LabelTP A) :=
+  l1 = p l2.
 
-  Definition wordZero (w: word 0): w = WO :=
-    shatter_word w.
+Local Open Scope string.
 
+Inductive UnitStep : Modules -> RegsT -> RegsT -> RuleLabelT -> Type :=
+| EmptyStep :
+    forall (regInits : list RegInitT)
+           (rules : list (Attribute (Action Void)))
+           (meths : list DefMethT)
+           (oRegs : RegsT),
+      M.InDomain oRegs (namesOf regInits) ->
+      UnitStep (Mod regInits rules meths) oRegs (M.empty _)
+               (Build_LabelTP None (M.empty _) (M.empty _))
+| SingleRule : 
+  forall (ruleName : string) (ruleBody : Action (Bit 0))
+         (regInits : list RegInitT)
+         (rules : list (Attribute (Action Void)))
+         (meths : list DefMethT),
+    In (ruleName :: ruleBody)%struct rules ->
+    forall (oRegs news : RegsT) (calls : CallsT)
+           (retV : type (Bit 0)),
+      SemAction oRegs (ruleBody type) news calls retV ->
+      M.InDomain oRegs (namesOf regInits) ->
+      UnitStep (Mod regInits rules meths) oRegs news
+               (Build_LabelTP (Some ruleName) (M.empty _) calls)
+| SingleMeth :
+    forall (regInits : list RegInitT)
+           (rules : list (Attribute (Action Void)))
+           (meths : list DefMethT)
+           (oRegs : RegsT)
+           (calls : CallsT) (news : RegsT) 
+           (meth : DefMethT),
+      In meth meths ->
+      forall (argV : type (arg (objType (attrType meth))))
+             (retV : type (ret (objType (attrType meth))))
+             (udefs : CallsT),
+        SemAction oRegs (objVal (attrType meth) type argV) news calls retV ->
+        udefs = M.add meth {|
+                        objType := objType (attrType meth);
+                        objVal := (argV, retV) |} (M.empty _) ->
+        M.InDomain oRegs (namesOf regInits) ->
+        UnitStep (Mod regInits rules meths) oRegs news
+                 (Build_LabelTP None udefs calls)
+| LeftIntro :
+    forall (m1 m2 : Modules)
+           (oRegs1 oRegs2 oRegs news : RegsT)
+           (l : RuleLabelT),
+      M.InDomain oRegs2 (namesOf (getRegInits m2)) ->
+      UnitStep m1 oRegs1 news l ->
+      oRegs = M.union oRegs1 oRegs2 ->
+      UnitStep (ConcatMod m1 m2) oRegs news l
+| RightIntro :
+    forall (m1 m2 : Modules)
+           (oRegs1 oRegs2 oRegs news : RegsT)
+           (l : RuleLabelT),
+      M.InDomain oRegs1 (namesOf (getRegInits m1)) ->
+      UnitStep m2 oRegs2 news l ->
+      oRegs = M.union oRegs1 oRegs2 ->
+      UnitStep (ConcatMod m1 m2) oRegs news l.
+
+Inductive UnitSteps (m : Modules) (o : RegsT) : RegsT -> RuleLabelT -> Type :=
+| UnitSteps1 : forall {u l}, UnitStep m o u l -> UnitSteps m o u l
+| UnitStepsUnion : forall {u1 u2 : RegsT} {l1 l2 : RuleLabelT}, 
+                     UnitSteps m o u1 l1 -> UnitSteps m o u2 l2 
+                     -> CanCombine (u1, l1) (u2, l2)
+                     -> UnitSteps m o (M.union u1 u2) (mergeLabel l1 l2).
+
+Definition signIsEq :
+  forall (l1 l2 : Typed SignT), sumbool (l1 = l2) (l1 <> l2).
+Proof.
+  intros. destruct l1, l2. 
+  destruct (SignatureT_dec objType objType0).
+  - induction e. destruct objType, objVal, objVal0.
+    destruct (isEq arg t t1). induction e.
+    destruct (isEq ret t0 t2). induction e. left. reflexivity.
+    right. unfold not. intros. apply typed_eq in H.
+    inversion H. apply n in H1. assumption.
+    right. unfold not. intros. apply typed_eq in H.
+    inversion H. apply n in H1. assumption.
+  - right. unfold not. intros. inversion H. apply n in H1.
+    assumption.
+Qed.
+
+Definition hide {A : Type} (l : LabelTP A) : LabelTP A :=
+  match l with
+      Build_LabelTP rm ds cs => 
+      Build_LabelTP rm (M.subtractKV signIsEq ds cs)
+                    (M.subtractKV signIsEq cs ds)
+  end.
+
+Definition wellHidden {A : Type} (l : LabelTP A) (m : Modules) :=
+  match l with
+      Build_LabelTP rm ds cs =>
+      M.NotOnDomain ds (getCmsMod m)
+      /\ M.NotOnDomain cs (getDmsMod m)
+  end.
+
+Inductive Step (m : Modules) (o u : RegsT) : RuleLabelT -> Type :=
+  MkStep : forall {l l': RuleLabelT},
+             UnitSteps m o u l ->
+             l' = hide l -> wellHidden l' m ->
+             Step m o u l'.
+
+Inductive MultiStep (m : Modules) (regs : RegsT) : RegsT -> list RuleLabelT -> Prop :=
+| MSNil : MultiStep m regs regs nil
+| MSMulti :
+    forall regs' labels,
+      MultiStep m regs regs' labels ->
+      forall l u,
+        Step m regs' u l ->
+        forall (regs'' : RegsT),
+          regs'' = M.update regs' u ->
+          MultiStep m regs regs'' (l :: labels).
+
+Section MakeMap.
   Variable A: Type.
+  Variable f1 f2: A -> Type.
+  Variable f: forall x, f1 x -> f2 x.
 
-  (* a lemma for wordVecDec *)
-  Definition wordVecDec':
-    forall n (f g: word n -> A), (forall x: word n, {f x = g x} + {f x <> g x}) ->
-                                 {forall x, f x = g x} + {exists x, f x <> g x}.
-  Proof.
-    intro n.
-    induction n; intros f g H.
-    - destruct (H WO).
-      + left; intros x.
-        rewrite (wordZero x) in *; intuition.
-      + right; eauto.
-    - assert (Hn: forall b (x: word n),
-                    {f (WS b x) = g (WS b x)} + {f (WS b x) <> g (WS b x)}) by
-             (intros; specialize (H (WS b x)); intuition).
-      destruct (IHn _ _ (Hn false)) as [ef | nf].
-      + destruct (IHn _ _ (Hn true)) as [et | nt].
-        * left; intros x.
-          specialize (ef (wtl x)).
-          specialize (et (wtl x)).
-          pose proof (shatter_word x) as use; simpl in *.
-          destruct (whd x); rewrite <- use in *; intuition.
-        * right; destruct_ex; eauto.
-      + right; destruct_ex; eauto.
-  Qed.
-
-  Definition wordVecDec:
-    forall n (f g: word n -> A), (forall x: word n, {f x = g x} + {f x <> g x}) ->
-                                 {f = g} + {f <> g}.
-  Proof.
-    intros.
-    pose proof (wordVecDec' _ _ H) as [lt | rt].
-    left; apply functional_extensionality; intuition.
-    right; unfold not; intros eq; rewrite eq in *.
-    destruct rt; intuition.
-  Qed.
-End WordFunc.
-
-Section VecFunc.
-  Variable A: Type.
-  Fixpoint evalVec n (vec: Vec A n): word n -> A.
-  Proof.
-    refine match vec in Vec _ n return word n -> A with
-             | Vec0 e => fun _ => e
-             | VecNext n' v1 v2 =>
-               fun w =>
-                 match w in word m0 return m0 = S n' -> A with
-                   | WO => _
-                   | WS b m w' =>
-                     if b
-                     then fun _ => evalVec _ v2 (_ w')
-                     else fun _ => evalVec _ v2 (_ w')
-                 end eq_refl
-           end;
-    clear evalVec.
-    abstract (intros; discriminate).
-    abstract (injection _H; intros; subst; intuition).
-    abstract (injection _H; intros; subst; intuition).
-  Defined.
-
-  Variable B: Type.
-  Variable map: A -> B.
-  Fixpoint mapVec n (vec: Vec A n): Vec B n :=
-    match vec in Vec _ n return Vec B n with
-      | Vec0 e => Vec0 (map e)
-      | VecNext n' v1 v2 => VecNext (mapVec v1) (mapVec v2)
-    end.
-End VecFunc.
-
-(* for any kind, we have decidable equality on its representation *)
-Definition isEq : forall k (e1: type k) (e2: type k),
-                    {e1 = e2} + {e1 <> e2}.
-Proof.
-  refine (fix isEq k : forall (e1: type k) (e2: type k), {e1 = e2} + {e1 <> e2} :=
-            match k return forall (e1: type k) (e2: type k),
-                             {e1 = e2} + {e1 <> e2} with
-              | Bool => bool_dec
-              | Bit n => fun e1 e2 => weq e1 e2
-              | Vector n nt =>
-                  fun e1 e2 =>
-                    wordVecDec e1 e2 (fun x => isEq _ (e1 x) (e2 x))
-              | Struct h =>
-                (fix isEqs atts : forall (vs1 vs2 : forall i, @GetAttrType _ (map (mapAttr type) atts) i),
-                                    {vs1 = vs2} + {vs1 <> vs2} :=
-                   match atts return forall (vs1 vs2 : forall i, @GetAttrType _ (map (mapAttr type) atts) i),
-                                       {vs1 = vs2} + {vs1 <> vs2} with
-                     | nil => fun _ _ => Yes
-                     | att :: atts' => fun vs1 vs2 =>
-                       isEq _
-                            (vs1 {| bindex := attrName att; indexb := {| ibound := 0;
-                                      boundi := eq_refl :
-                                                  nth_error
-                                                    (map (attrName (Kind:=Type))
-                                                         (map (mapAttr type) (att :: atts'))) 0
-                                                    = Some (attrName att) |} |})
-                            (vs2 {| bindex := attrName att; indexb := {| ibound := 0;
-                                      boundi := eq_refl :
-                                                  nth_error
-                                                    (map (attrName (Kind:=Type))
-                                                         (map (mapAttr type) (att :: atts'))) 0
-                                                    = Some (attrName att) |} |});;
-                       isEqs atts'
-                       (fun i => vs1 {| indexb := {| ibound := S (ibound (indexb i)) |} |})
-                       (fun i => vs2 {| indexb := {| ibound := S (ibound (indexb i)) |} |});;
-                       Yes
-                   end) h
-            end); clear isEq; try clear isEqs;
-  abstract (unfold BoundedIndexFull in *; simpl in *; try (intro; subst; tauto);
-  repeat match goal with
-           | [ |- _ = _ ] => extensionality i
-           | [ x : BoundedIndex _ |- _ ] => destruct x
-           | [ x : IndexBound _ _ |- _ ] => destruct x
-           | [ H : nth_error nil ?n = Some _ |- _ ] => destruct n; discriminate
-           | [ |- _ {| indexb := {| ibound := ?b |} |} = _ ] =>
-             match goal with
-               | [ x : _ |- _ ] =>
-                 match x with
-                   | b => destruct b; simpl in *
-                 end
-             end
-           | [ H : Specif.value _ = Some _ |- _ ] => progress (injection H; intro; subst)
-           | [ H : _ = _ |- _ ] => progress rewrite (UIP_refl _ _ H)
-           | [ H : _ = _ |- _ {| bindex := ?bi; indexb := {| ibound := S ?ib; boundi := ?pf |} |} = _ ] =>
-             apply (f_equal (fun f => f {| bindex := bi; indexb := {| ibound := ib; boundi := pf |} |})) in H
-         end; auto).
-Defined.
-
-Definition evalUniBool (op: UniBoolOp) : bool -> bool :=
-  match op with
-    | Neg => negb
-  end.
-
-Definition evalBinBool (op: BinBoolOp) : bool -> bool -> bool :=
-  match op with
-    | And => andb
-    | Or => orb
-  end.
-
-(* the head of a word, or false if the word has 0 bits *)
-Definition whd' sz (w: word sz) :=
-  match sz as s return word s -> bool with
-    | 0 => fun _ => false
-    | S n => fun w => whd w
-  end w.
-
-Definition evalUniBit n1 n2 (op: UniBitOp n1 n2): word n1 -> word n2.
-refine match op with
-         | Inv n => @wneg n
-         | ConstExtract n1 n2 n3 => fun w => split2 n1 n2 (split1 (n1 + n2) n3 w)
-         | ZeroExtendTrunc n1 n2 => fun w => split2 n1 n2 (_ (combine (wzero n2) w))
-         | SignExtendTrunc n1 n2 => fun w => split2 n1 n2 (_ (combine (if whd' w
-                                                                       then wones n2
-                                                                       else wzero n2) w))
-         | TruncLsb n1 n2 => fun w => split1 n1 n2 w
-       end;
-  assert (H: n3 + n0 = n0 + n3) by omega;
-  rewrite H in *; intuition.
-Defined.
-
-Definition evalBinBit n1 n2 n3 (op: BinBitOp n1 n2 n3)
-  : word n1 -> word n2 -> word n3 :=
-  match op with
-    | Add n => @wplus n
-    | Sub n => @wminus n
-  end.
-
-Definition evalConstStruct attrs (ils : ilist (fun a => type (attrType a)) attrs) : type (Struct attrs) :=
-  fun (i: BoundedIndex (namesOf (map (mapAttr type) attrs))) =>
-    mapAttrEq1 type attrs i
-               (ith_Bounded _ ils (getNewIdx1 type attrs i)).
-
-(* evaluate any constant operation *)
-Fixpoint evalConstT k (e: ConstT k): type k :=
-  match e in ConstT k return type k with
-    | ConstBool b => b
-    | ConstBit n w => w
-    | ConstVector k' n v => evalVec (mapVec (@evalConstT k') v)
-    | ConstStruct attrs ils => evalConstStruct (imap _ (fun _ ba => evalConstT ba) ils)
-  end.
-
-Definition evalConstFullT k (e: ConstFullT k) :=
-  match e in ConstFullT k return fullType type k with
-    | SyntaxConst k' c' => evalConstT c'
-    | NativeConst t c c' => c'
-  end.
-
-(* maps register names to the values which they currently hold *)
-Definition RegsT := M.t (Typed (fullType type)).
-
-(* a pair of the value sent to a method call and the value it returned *)
-Definition SignT k := (type (arg k) * type (ret k))%type.
-
-(* a list of simulatenous method call actions made during a single step *)
-Definition CallsT := M.t (Typed SignT).
-
-Section Semantics.
-  Definition mkStruct attrs (ils : ilist (fun a => type (attrType a)) attrs) : type (Struct attrs) :=
-    fun (i: BoundedIndex (namesOf (map (mapAttr type) attrs))) =>
-      mapAttrEq1 type attrs i (ith_Bounded _ ils (getNewIdx1 type attrs i)).
-
-  Fixpoint evalExpr exprT (e: Expr type exprT): fullType type exprT :=
-    match e in Expr _ exprT return fullType type exprT with
-      | Var _ v => v
-      | Const _ v => evalConstT v
-      | UniBool op e1 => (evalUniBool op) (evalExpr e1)
-      | BinBool op e1 e2 => (evalBinBool op) (evalExpr e1) (evalExpr e2)
-      | UniBit n1 n2 op e1 => (evalUniBit op) (evalExpr e1)
-      | BinBit n1 n2 n3 op e1 e2 => (evalBinBit op) (evalExpr e1) (evalExpr e2)
-      | ITE _ p e1 e2 => if evalExpr p
-                         then evalExpr e1
-                         else evalExpr e2
-      | Eq _ e1 e2 => if isEq _ (evalExpr e1) (evalExpr e2)
-                      then true
-                      else false
-      | ReadIndex _ _ i f => (evalExpr f) (evalExpr i)
-      | ReadField heading fld val =>
-          mapAttrEq2 type fld
-            ((evalExpr val) (getNewIdx2 type fld))
-      | BuildVector _ k vec => evalVec (mapVec (@evalExpr _) vec)
-      | BuildStruct attrs ils => mkStruct (imap _ (fun _ ba => evalExpr ba) ils)
-      | UpdateVector _ _ fn i v =>
-          fun w => if weq w (evalExpr i) then evalExpr v else (evalExpr fn) w
-    end.
-
-  (*register names and constant expressions for their initial values *)
-  Variable regInit: list RegInitT.
-
-  Variable rules: list (Attribute (Action (Bit 0))).
-
-  (* register values just before the current cycle *)
-  Variable oldRegs: RegsT.
-
-  Inductive SemAction:
-    forall k, ActionT type k -> RegsT -> CallsT -> type k -> Prop :=
-  | SemMCall
-      meth s (marg: Expr type (SyntaxKind (arg s)))
-      (mret: type (ret s))
-      retK (fret: type retK)
-      (cont: type (ret s) -> ActionT type retK)
-      newRegs (calls: CallsT) acalls
-      (HAcalls: acalls = M.add meth {| objVal := (evalExpr marg, mret) |} calls)
-      (HSemAction: SemAction (cont mret) newRegs calls fret):
-      SemAction (MCall meth s marg cont) newRegs acalls fret
-  | SemLet
-      k (e: Expr type k) retK (fret: type retK)
-      (cont: fullType type k -> ActionT type retK) newRegs calls
-      (HSemAction: SemAction (cont (evalExpr e)) newRegs calls fret):
-      SemAction (Let_ e cont) newRegs calls fret
-  | SemReadReg
-      (r: string) regT (regV: fullType type regT)
-      retK (fret: type retK) (cont: fullType type regT -> ActionT type retK)
-      newRegs calls
-      (HRegVal: M.find r oldRegs = Some {| objType := regT; objVal := regV |})
-      (HSemAction: SemAction (cont regV) newRegs calls fret):
-      SemAction (ReadReg r _ cont) newRegs calls fret
-  | SemWriteReg
-      (r: string) k
-      (e: Expr type k)
-      retK (fret: type retK)
-      (cont: ActionT type retK) newRegs calls anewRegs
-      (HANewRegs: anewRegs = M.add r {| objVal := (evalExpr e) |} newRegs)
-      (HSemAction: SemAction cont newRegs calls fret):
-      SemAction (WriteReg r e cont) anewRegs calls fret
-  | SemIfElseTrue
-      (p: Expr type (SyntaxKind Bool)) k1
-      (a: ActionT type k1)
-      (a': ActionT type k1)
-      (r1: type k1)
-      k2 (cont: type k1 -> ActionT type k2)
-      newRegs1 newRegs2 calls1 calls2 (r2: type k2)
-      (HTrue: evalExpr p = true)
-      (HAction: SemAction a newRegs1 calls1 r1)
-      (HSemAction: SemAction (cont r1) newRegs2 calls2 r2)
-      unewRegs ucalls
-      (HUNewRegs: unewRegs = MF.union newRegs1 newRegs2)
-      (HUCalls: ucalls = MF.union calls1 calls2):
-      SemAction (IfElse p a a' cont) unewRegs ucalls r2
-  | SemIfElseFalse
-      (p: Expr type (SyntaxKind Bool)) k1
-      (a: ActionT type k1)
-      (a': ActionT type k1)
-      (r1: type k1)
-      k2 (cont: type k1 -> ActionT type k2)
-      newRegs1 newRegs2 calls1 calls2 (r2: type k2)
-      (HFalse: evalExpr p = false)
-      (HAction: SemAction a' newRegs1 calls1 r1)
-      (HSemAction: SemAction (cont r1) newRegs2 calls2 r2)
-      unewRegs ucalls
-      (HUNewRegs: unewRegs = MF.union newRegs1 newRegs2)
-      (HUCalls: ucalls = MF.union calls1 calls2):
-      SemAction (IfElse p a a' cont) unewRegs ucalls r2
-  | SemAssertTrue
-      (p: Expr type (SyntaxKind Bool)) k2
-      (cont: ActionT type k2) newRegs2 calls2 (r2: type k2)
-      (HTrue: evalExpr p = true)
-      (HSemAction: SemAction cont newRegs2 calls2 r2):
-      SemAction (Assert_ p cont) newRegs2 calls2 r2
-  | SemReturn
-      k (e: Expr type (SyntaxKind k)) evale
-      (HEvalE: evale = evalExpr e):
-      SemAction (Return e) (M.empty _) (M.empty _) evale.
-
-  Theorem inversionSemAction
-          k a news calls retC
-          (evalA: @SemAction k a news calls retC):
-    match a with
-      | MCall m s e c =>
-        exists mret pcalls,
-          SemAction (c mret) news pcalls retC /\
-          calls = M.add m {| objVal := (evalExpr e, mret) |} pcalls
-      | Let_ _ e cont =>
-        SemAction (cont (evalExpr e)) news calls retC
-      | ReadReg r k c =>
-        exists rv,
-          M.find r oldRegs = Some {| objType := k; objVal := rv |} /\
-          SemAction (c rv) news calls retC
-      | WriteReg r _ e a =>
-        exists pnews,
-          SemAction a pnews calls retC /\
-          news = M.add r {| objVal := evalExpr e |} pnews
-      | IfElse p _ aT aF c =>
-        exists news1 calls1 news2 calls2 r1,
-          match evalExpr p with
-            | true =>
-              SemAction aT news1 calls1 r1 /\
-              SemAction (c r1) news2 calls2 retC /\
-              news = MF.union news1 news2 /\
-              calls = MF.union calls1 calls2
-            | false =>
-              SemAction aF news1 calls1 r1 /\
-              SemAction (c r1) news2 calls2 retC /\
-              news = MF.union news1 news2 /\
-              calls = MF.union calls1 calls2
-          end
-      | Assert_ e c =>
-        SemAction c news calls retC /\
-        evalExpr e = true
-      | Return e =>
-        retC = evalExpr e /\
-        news = M.empty _ /\
-        calls = M.empty _
-    end.
-  Proof.
-    destruct evalA; eauto; repeat eexists; destruct (evalExpr p); eauto; try discriminate.
-  Qed.
-
-  Inductive SemMod: option string -> RegsT -> list DefMethT -> CallsT -> CallsT -> Prop :=
-  | SemEmpty news meths dm cm
-             (HEmptyRegs: news = M.empty _)
-             (HEmptyDms: dm = M.empty _)
-             (HEmptyCms: cm = M.empty _):
-      SemMod None news meths dm cm
-  | SemAddRule (ruleName: string)
-               (ruleBody: Action (Bit 0))
-               (HInRule: In {| attrName := ruleName; attrType := ruleBody |} rules)
-               news calls retV
-               (HAction: SemAction (ruleBody type) news calls retV)
-               news2 meths dm2 cm2
-               (HSemMod: SemMod None news2 meths dm2 cm2)
-               (HNoDoubleWrites: MF.Disj news news2)
-               (HNoCallsBoth: MF.Disj calls cm2)
-               unews ucalls
-               (HRegs: unews = MF.union news news2)
-               (HCalls: ucalls = MF.union calls cm2):
-      SemMod (Some ruleName) unews meths dm2 ucalls
-  (* method `meth` was also called this clock cycle *)
-  | SemAddMeth calls news (meth: DefMethT) meths argV retV
-               (HIn: In meth meths)
-               (HAction: SemAction ((objVal (attrType meth)) type argV) news calls retV)
-               news2 dm2 cm2
-               (HSemMod: SemMod None news2 meths dm2 cm2)
-               (HNoDoubleWrites: MF.Disj news news2)
-               (HNoCallsBoth: MF.Disj calls cm2)
-               unews ucalls udefs
-               (HRegs: unews = MF.union news news2)
-               (HCalls: ucalls = MF.union calls cm2)
-               (HNew: M.find (attrName meth) dm2 = None)
-               (HDefs: udefs = M.add (attrName meth) {| objVal := (argV, retV) |} dm2):
-      SemMod None unews meths udefs ucalls.
-
-End Semantics.
-
-Ltac cheap_firstorder :=
-  repeat match goal with
-           | [ H : ex _ |- _ ] => destruct H
-           | [ H : _ /\ _ |- _ ] => destruct H
-         end.
-
-Ltac invertAction H := apply inversionSemAction in H; simpl in H; cheap_firstorder; try subst.
-Ltac invertActionFirst :=
-  match goal with
-    | [H: SemAction _ _ _ _ _ |- _] => invertAction H
-  end.
-Ltac invertActionRep :=
-  repeat
-    match goal with
-      | [H: SemAction _ _ _ _ _ |- _] => invertAction H
-      | [H: if ?c
-            then
-              SemAction _ _ _ _ _ /\ _ /\ _ /\ _
-            else
-              SemAction _ _ _ _ _ /\ _ /\ _ /\ _ |- _] =>
-        let ic := fresh "ic" in
-        (remember c as ic; destruct ic; dest; subst)
-    end.
-
-Ltac invertSemMod H :=
-  inv H;
-  repeat match goal with
-           | [H: MF.Disj _ _ |- _] => clear H
-         end.
-
-Ltac invertSemModRep :=
-  repeat
-    match goal with
-      | [H: SemMod _ _ _ _ _ _ _ |- _] => invertSemMod H
-    end.
-
-Lemma SemAction_olds_ext:
-  forall retK a olds1 olds2 news calls (retV: type retK),
-    MF.Sub olds1 olds2 ->
-    SemAction olds1 a news calls retV ->
-    SemAction olds2 a news calls retV.
-Proof.
-  induction a; intros.
-  - invertAction H1; econstructor; eauto.
-  - invertAction H1; econstructor; eauto.
-  - invertAction H1; econstructor; eauto.
-    apply M.find_1. apply H0. apply MF.F.P.F.find_mapsto_iff. assumption.
-  - invertAction H0; econstructor; eauto.
-  - invertAction H1.
-    remember (evalExpr e) as cv; destruct cv; dest.
-    + eapply SemIfElseTrue; eauto.
-    + eapply SemIfElseFalse; eauto.
-  - invertAction H0; econstructor; eauto.
-  - invertAction H0; econstructor; eauto.
-Qed.
-
-Lemma SemMod_empty:
-  forall rules or dms, SemMod rules or None (M.empty _) dms (M.empty _) (M.empty _).
-Proof. intros; apply SemEmpty; auto. Qed.
-
-Lemma SemMod_empty_inv:
-  forall rules or nr dms cmMap,
-    SemMod rules or None nr dms (M.empty _) cmMap ->
-    nr = M.empty _ /\ cmMap = M.empty _.
-Proof.
-  intros; inv H; [intuition|].
-  apply @Equal_val with (k:= meth) in HDefs.
-  rewrite MF.find_add_1 in HDefs.
-  rewrite MF.find_empty in HDefs. inv HDefs.
-Qed.
-
-Lemma SemMod_olds_ext:
-  forall rules or1 or2 rm nr dms dmMap cmMap,
-    MF.Sub or1 or2 -> SemMod rules or1 rm nr dms dmMap cmMap ->
-    SemMod rules or2 rm nr dms dmMap cmMap.
-Proof.
-  induction 2; intros.
-  - subst; constructor; auto.
-  - eapply SemAddRule; eauto.
-    eapply SemAction_olds_ext; eauto.
-  - eapply SemAddMeth; eauto.
-    eapply SemAction_olds_ext; eauto.
-Qed.
-
-Lemma SemMod_dmMap_InDomain:
-  forall rules dms or rm nr dmMap cmMap,
-    SemMod rules or rm nr dms dmMap cmMap ->
-    MF.InDomain dmMap (namesOf dms).
-Proof.
-  induction 1; intros; subst; intuition.
-  unfold MF.InDomain. intros.
-  apply MF.F.P.F.empty_in_iff in H. contradiction.
-  apply MF.InDomain_add; auto.
-  apply in_map; auto.
-Qed.
-
-Lemma SemMod_rule_singleton:
-  forall dms rules olds news r rb cmMap (Hrb: Some rb = getAttribute r rules)
-         (Hwf: NoDup (namesOf rules))
-         (Hsem: SemMod rules olds (Some r) news dms (M.empty _) cmMap),
-    SemAction olds (attrType rb type) news cmMap WO.
-Proof.
-  admit.
-Qed.
-
-Lemma SemMod_meth_singleton:
-  forall dms rules olds news dm a (Ha: Some a = getAttribute dm dms)
-         argV retV cmMap
-         (Hwf: NoDup (namesOf dms))
-         (Hsem: SemMod rules olds None news dms
-                       (M.add dm
-                            {| objType := objType (attrType a);
-                               objVal := (argV, retV) |} (M.empty _)) cmMap),
-    SemAction olds (objVal (attrType a) type argV) news cmMap retV.
-Proof.
-  admit.
-Qed.
-
-Lemma SemMod_dms_cut:
-  forall dms2 rules dms1 or rm nr dmMap cmMap,
-    SemMod rules or rm nr dms1 dmMap cmMap ->
-    MF.InDomain dmMap (namesOf dms2) -> (forall k, In k dms2 -> In k dms1) -> 
-    SemMod rules or rm nr dms2 dmMap cmMap.
-Proof.
-  admit.
-Qed.
-
-Lemma SemMod_dms_ext:
-  forall dms2 rules dms1 or rm nr dmMap cmMap,
-    SemMod rules or rm nr dms1 dmMap cmMap ->
-    (forall k, In k dms1 -> In k dms2) ->
-    SemMod rules or rm nr dms2 dmMap cmMap.
-Proof.
-  admit.
-Qed.
-
-Lemma SemMod_dms_free:
-  forall rules dms1 dms2 or rm nr cmMap,
-    SemMod rules or rm nr dms1 (M.empty _) cmMap ->
-    SemMod rules or rm nr dms2 (M.empty _) cmMap.
-Proof.
-  admit.
-Qed.
-
-Lemma SemMod_rules_free:
-  forall rules1 rules2 dms or nr dmMap cmMap,
-    SemMod rules1 or None nr dms dmMap cmMap ->
-    SemMod rules2 or None nr dms dmMap cmMap.
-Proof.
-  admit.
-Qed.
-
-Lemma SemMod_rules_ext:
-  forall rules1 rules2 r dms or nr dmMap cmMap,
-    SemMod rules1 or (Some r) nr dms dmMap cmMap ->
-    SubList rules1 rules2 ->
-    SemMod rules2 or (Some r) nr dms dmMap cmMap.
-Proof.
-  admit.
-Qed.
-
-Lemma SemMod_div:
-  forall rules olds rm news dms dmMap1 dmMap2 cmMap
-         (Hsem: SemMod rules olds rm news dms (MF.union dmMap1 dmMap2) cmMap)
-         (Hdisj: MF.Disj dmMap1 dmMap2),
-  exists news1 news2 cmMap1 cmMap2,
-    MF.Disj news1 news2 /\ news = MF.union news1 news2 /\
-    MF.Disj cmMap1 cmMap2 /\ cmMap = MF.union cmMap1 cmMap2 /\
-    SemMod rules olds rm news1 dms dmMap1 cmMap1 /\
-    SemMod rules olds None news2 dms dmMap2 cmMap2.
-Proof.
-  admit.
-Qed.
-
-Lemma SemMod_merge_meths:
-  forall rules dms or nr1 nr2 dmMap1 dmMap2 cmMap1 cmMap2,
-    SemMod rules or None nr1 dms dmMap1 cmMap1 ->
-    SemMod rules or None nr2 dms dmMap2 cmMap2 ->
-    MF.Disj nr1 nr2 -> MF.Disj dmMap1 dmMap2 -> MF.Disj cmMap1 cmMap2 ->
-    SemMod rules or None (MF.union nr1 nr2) dms (MF.union dmMap1 dmMap2) (MF.union cmMap1 cmMap2).
-Proof.
-  admit.
-Qed.
-
-Lemma SemMod_merge_rule:
-  forall rules dms or r nr1 nr2 dmMap1 dmMap2 cmMap1 cmMap2,
-    SemMod rules or (Some r) nr1 dms dmMap1 cmMap1 ->
-    SemMod rules or None nr2 dms dmMap2 cmMap2 ->
-    MF.Disj nr1 nr2 -> MF.Disj dmMap1 dmMap2 -> MF.Disj cmMap1 cmMap2 ->
-    SemMod rules or (Some r) (MF.union nr1 nr2) dms (MF.union dmMap1 dmMap2) (MF.union cmMap1 cmMap2).
-Proof.
-  admit.
-Qed.
-
-(* dm       : defined methods
-   cm       : called methods
-   ruleMeth : `None` if it is a method,
-              `Some [rulename]` if it is a rule *)
-Record RuleLabelT := { ruleMeth: option string;
-                       dms: list string;
-                       dmMap: CallsT;
-                       cms: list string;
-                       cmMap: CallsT }.
-
-Hint Unfold ruleMeth dms dmMap cms cmMap.
-
-Definition CombineRm (rm1 rm2 crm: option string) :=
-  (rm1 = None \/ rm2 = None) /\
-  crm = match rm1, rm2 with
-          | Some rn1, None => Some rn1
-          | None, Some rn2 => Some rn2
-          | _, _ => None
-        end.
-
-Lemma combineRm_prop_1:
-  forall r1 rm2 cr (Hcrm: CombineRm (Some r1) rm2 (Some cr)),
-    r1 = cr.
-Proof.
-  intros; unfold CombineRm in Hcrm; dest.
-  destruct rm2; inv H0; reflexivity.
-Qed.
-
-Lemma combineRm_prop_2:
-  forall rm1 r2 cr (Hcrm: CombineRm rm1 (Some r2) (Some cr)),
-    r2 = cr.
-Proof.
-  intros; unfold CombineRm in Hcrm; dest.
-  destruct rm1; inv H0; reflexivity.
-Qed.
-
-Lemma combineRm_prop_3:
-  forall rm1 crm (Hcrm: CombineRm rm1 None crm),
-    rm1 = crm.
-Proof.
-  intros; unfold CombineRm in Hcrm; dest.
-  destruct rm1; inv H0; reflexivity.
-Qed.
-
-Lemma combineRm_prop_4:
-  forall rm2 crm (Hcrm: CombineRm None rm2 crm),
-    rm2 = crm.
-Proof.
-  intros; unfold CombineRm in Hcrm; dest.
-  destruct rm2; inv H0; reflexivity.
-Qed.
-
-Lemma combineRm_prop_5:
-  forall rm1 rm2 (Hcrm: CombineRm rm1 rm2 None),
-    rm1 = None /\ rm2 = None.
-Proof.
-  intros; unfold CombineRm in Hcrm; dest.
-  destruct rm1, rm2; intuition; inv H1.
-Qed.
-
-Definition CallIffDef (l1 l2: RuleLabelT) :=
-  (forall m, In m (cms l1) -> In m (dms l2) -> M.find m (cmMap l1) = M.find m (dmMap l2)) /\
-  (forall m, In m (cms l2) -> In m (dms l1) -> M.find m (dmMap l1) = M.find m (cmMap l2)).
-
-Definition FiltDm (l1 l2 l: RuleLabelT) :=
-  dmMap l = MF.union (MF.complement (dmMap l1) (cms l2)) (MF.complement (dmMap l2) (cms l1)).
-
-Definition FiltCm (l1 l2 l: RuleLabelT) :=
-  cmMap l = MF.union (MF.complement (cmMap l1) (dms l2)) (MF.complement (cmMap l2) (dms l1)).
-
-Definition ConcatLabel (l1 l2 l: RuleLabelT) :=
-  CombineRm (ruleMeth l1) (ruleMeth l2) (ruleMeth l) /\
-  CallIffDef l1 l2 /\ FiltDm l1 l2 l /\ FiltCm l1 l2 l.
-
-Hint Unfold CombineRm CallIffDef FiltDm FiltCm ConcatLabel.
-
-Ltac destConcatLabel :=
-  repeat match goal with
-           | [H: ConcatLabel _ _ _ |- _] =>
-             let Hcrm := fresh "Hcrm" in
-             let Hcid := fresh "Hcid" in
-             let Hfd := fresh "Hfd" in
-             let Hfc := fresh "Hfc" in
-             destruct H as [Hcrm [Hcid [Hfd Hfc]]]; clear H; dest;
-             unfold ruleMeth in Hcrm
-         end.
-
-(* rm = ruleMethod *)
-Inductive LtsStep:
-  Modules -> option string -> RegsT -> RegsT -> CallsT -> CallsT -> Prop :=
-| LtsStepMod regInits oRegs nRegs rules meths rm dmMap cmMap
-             (HOldRegs: MF.InDomain oRegs (namesOf regInits))
-             (Hltsmod: SemMod rules oRegs rm nRegs meths dmMap cmMap):
-    LtsStep (Mod regInits rules meths) rm oRegs nRegs dmMap cmMap
-| LtsStepConcat m1 rm1 olds1 news1 dmMap1 cmMap1
-                m2 rm2 olds2 news2 dmMap2 cmMap2
-                (HOldRegs1: MF.InDomain olds1 (namesOf (getRegInits m1)))
-                (HOldRegs2: MF.InDomain olds2 (namesOf (getRegInits m2)))
-                (Hlts1: @LtsStep m1 rm1 olds1 news1 dmMap1 cmMap1)
-                (Hlts2: @LtsStep m2 rm2 olds2 news2 dmMap2 cmMap2)
-                crm colds cnews cdmMap ccmMap
-                (Holds: colds = MF.union olds1 olds2)
-                (Hnews: cnews = MF.union news1 news2)
-                (HdmMap: MF.Disj dmMap1 dmMap2)
-                (HcmMap: MF.Disj cmMap1 cmMap2)
-                (HMerge: ConcatLabel
-                           (Build_RuleLabelT rm1 (getDmsMod m1) dmMap1 (getCmsMod m1) cmMap1)
-                           (Build_RuleLabelT rm2 (getDmsMod m2) dmMap2 (getCmsMod m2) cmMap2)
-                           (Build_RuleLabelT crm (getDmsMod (ConcatMod m1 m2)) cdmMap
-                                             (getCmsMod (ConcatMod m1 m2)) ccmMap)):
-    LtsStep (ConcatMod m1 m2) crm colds cnews cdmMap ccmMap.
-
-Lemma ltsStep_rule:
-  forall m rm r or nr dmMap cmMap
-         (Hstep: LtsStep m rm or nr dmMap cmMap)
-         (Hrm: rm = Some r),
-    In r (namesOf (getRules m)).
-Proof.
-  intros; subst.
-  dependent induction Hstep.
-  - invertSemMod Hltsmod.
-    apply in_map_iff; simpl; eexists; split; [|eassumption]; reflexivity.
-  - simpl; destConcatLabel.
-    unfold CombineRm in Hcrm; dest.
-    destruct rm1, rm2.
-    + destruct H; discriminate.
-    + inv H0; specialize (IHHstep1 s eq_refl).
-      unfold namesOf; rewrite map_app; apply in_or_app; left; assumption.
-    + inv H0; specialize (IHHstep2 s eq_refl).
-      unfold namesOf; rewrite map_app; apply in_or_app; right; assumption.
-    + inv H0.
-Qed.
-
-Ltac constr_concatMod :=
-  repeat autounfold with ModuleDefs;
-  match goal with
-    | [ |- LtsStep (ConcatMod ?m1 ?m2) (Some ?r) ?or _ _ _ ] =>
-      (let Hvoid := fresh "Hvoid" in
-       assert (In r (namesOf (getRules m1))) as Hvoid by in_tac;
-       clear Hvoid;
-       eapply LtsStepConcat with
-       (olds1 := MF.restrict or (namesOf (getRegInits m1)))
-         (olds2 := MF.complement or (namesOf (getRegInits m1)))
-         (rm1 := Some r) (rm2 := None); eauto)
-        || (eapply LtsStepConcat with
-            (olds1 := MF.restrict or (namesOf (getRegInits m1)))
-              (olds2 := MF.complement or (namesOf (getRegInits m1)))
-              (rm1 := None) (rm2 := Some r); eauto)
-    | [ |- LtsStep (ConcatMod ?m1 ?m2) None _ _ _ _ ] =>
-      eapply LtsStepConcat with
-      (olds1 := MF.restrict or (namesOf (getRegInits m1)))
-        (olds2 := MF.complement or (namesOf (getRegInits m1)))
-        (rm1 := None) (rm2 := None); eauto
-  end.
-
-Hint Extern 1 (LtsStep (Mod _ _ _) _ _ _ _ _) => econstructor.
-Hint Extern 1 (LtsStep (ConcatMod _ _) _ _ _ _ _) => constr_concatMod.
-Hint Extern 1 (SemMod _ _ _ _ _ _ _) => econstructor.
-(* Hint Extern 1 (SemAction _ _ _ _ _) => econstructor. *)
-Hint Extern 1 (SemAction _ (Return _) _ _ _) =>
-match goal with
-  | [ |- SemAction _ _ _ _ ?ret ] =>
-    match type of ret with
-      | type (Bit 0) => eapply SemReturn with (evale := WO)
-      | _ => econstructor
-    end
-end.
+  Fixpoint makeMap (l: list (Attribute (Typed f1))) : M.t (Typed f2) :=
+    match l with
+      | nil => M.empty _
+      | {| attrName := n; attrType := {| objVal := rv |} |} :: xs =>
+        M.add n {| objVal := f rv |} (makeMap xs)
+    end.  
+End MakeMap.
 
 Definition initRegs (init: list RegInitT): RegsT := makeMap (fullType type) evalConstFullT init.
 Hint Unfold initRegs.
 
-(* m = module
-   or = old registers
-   nr = new registers *)
+Inductive Behavior (m : Modules) : RegsT -> list LabelT -> Prop :=
+  MkBehavior :
+    forall newRegs labels labels',
+      MultiStep m (initRegs (getRegInits m)) newRegs labels ->
+      labels' = (List.map (mapLabelTP (fun _ => I)) labels) ->
+      Behavior m newRegs labels'.
 
-Definition update {A : Type} (m1 m2 : M.t A) := MF.union m2 m1.
+Definition TraceRefines (mimpl mspec : Modules) (f : LabelT -> LabelT) :=
+  forall simp limp,        Behavior mimpl simp         limp ->
+  exists (sspec : RegsT),  Behavior mspec sspec (map f limp).
 
-Inductive LtsStepClosure:
-  Modules ->
-  RegsT -> list RuleLabelT ->
-  Prop :=
-| lcNil m inits
-        (Hinits: inits = (initRegs (getRegInits m))):
-    LtsStepClosure m inits nil
-| lcLtsStep m rm or nr c cNew dNew or'
-            (Hlc: LtsStepClosure m or c)
-            (Hlts: LtsStep m rm or nr dNew cNew)
-            (Hrs: or' = update or nr):
-    LtsStepClosure m or' ((Build_RuleLabelT rm (getDmsMod m) dNew (getCmsMod m) cNew) :: c).
+Section Decomposition.
+  Variable rulesImp rulesSpec: list string.
+  Variable dmsImp dmsSpec: list DefMethT.
+  Variable imp spec: Modules.
+  Variable stateMap: RegsT -> RegsT.
+  Variable ruleMap: string -> string.
+  Variable p : (CallsT * CallsT) -> (CallsT * CallsT).
 
-Inductive ConcatLabelSeq: list RuleLabelT -> list RuleLabelT -> list RuleLabelT -> Prop :=
-| ConcatNil: ConcatLabelSeq nil nil nil
-| ConcatJoin l1 l2 l:
-    ConcatLabelSeq l1 l2 l ->
-    forall a1 a2 a, ConcatLabel a1 a2 a -> ConcatLabelSeq (a1 :: l1) (a2 :: l2) (a :: l).
+  Definition pMod {A : Type} (f : A -> A) (l : LabelTP A) : LabelTP A
+    := match l with
+    | Build_LabelTP rm dm cm => let (dm', cm') := p (dm, cm) in
+       Build_LabelTP (option_map f rm) dm' cm'
+    end.
 
-Definition RegsInDomain m :=
-  forall rm or nr dm cm,
-    LtsStep m rm or nr dm cm -> MF.InDomain nr (namesOf (getRegInits m)).
+  Definition pRL := pMod ruleMap.
 
-Lemma concatMod_RegsInDomain:
-  forall m1 m2 (Hin1: RegsInDomain m1) (Hin2: RegsInDomain m2),
-    RegsInDomain (ConcatMod m1 m2).
-Proof.
-  unfold RegsInDomain; intros; inv H.
-  specialize (Hin1 _ _ _ _ _ Hlts1).
-  specialize (Hin2 _ _ _ _ _ Hlts2).
-  clear -Hin1 Hin2.
-  unfold getRegInits, namesOf; rewrite map_app.
-  unfold MF.InDomain in *; intros.
-  repeat autounfold with MapDefs in H.
-  specialize (Hin1 k); specialize (Hin2 k).
-  apply MF.union_In in H.
-  destruct H; apply in_or_app; intuition auto.
-Qed.
+  Hypothesis pmerge : forall (ds1 ds2 cs1 cs2 : CallsT) (rm1 rm2 : option string)
+    , let l1 := Build_LabelTP rm1 ds1 cs1 in 
+      let l2 := Build_LabelTP rm2 ds2 cs2 in
+       M.Disj ds1 ds2 -> M.Disj cs1 cs2
+     -> NotBothRule rm1 rm2
+     -> mergeLabel (pRL l1) (pRL l2) = pRL (mergeLabel l1 l2).
 
-Section Domain.
-  Variable m: Modules.
-  Variable newRegsDomain: RegsInDomain m.
-  Theorem regsDomain r l
-    (clos: LtsStepClosure m r l):
-    MF.InDomain r (namesOf (getRegInits m)).
-  Proof.
-    induction clos.
-    - unfold MF.InDomain, initRegs in *; intros.
-      subst.
-      clear -H.
-      induction (getRegInits m); simpl in *.
-      + apply MF.F.P.F.empty_in_iff in H. assumption.
-      + destruct a; destruct attrType; simpl in *.
-        destruct (string_dec attrName k); intuition auto.
-        right. apply IHl.
-        rewrite MF.F.P.F.add_in_iff in H.
-        destruct H. specialize (n H). contradiction. assumption.
-    - pose proof (@newRegsDomain _ _ _ _ _ Hlts).
-      rewrite Hrs. unfold update.
-      apply MF.InDomain_union; intuition.
+  Hypothesis phide : forall (l : RuleLabelT), pRL (hide l) = hide (pRL l).
+
+  Hypothesis pwellHidden : forall (l : RuleLabelT), 
+   wellHidden (hide l) imp -> wellHidden (pRL (hide l)) spec.
+
+  Variable T : forall {oImp nImp lImp}, UnitStep imp oImp nImp lImp 
+             -> (RegsT * RuleLabelT).
+
+  Fixpoint Ts {oImp nImp lImp} (steps : UnitSteps imp oImp nImp lImp)
+      : RegsT * RuleLabelT
+      := match steps with
+    | UnitSteps1 _ _ step => T step
+    | UnitStepsUnion _ _ _ _ step1 step2 canCombine => 
+      let (u1, l1) := Ts step1 in
+      let (u2, l2) := Ts step2 in
+      (M.union u1 u2, mergeLabel l1 l2)
+    end.
+
+  Let Ts' {oImp nImp lImp} (step : Step imp oImp nImp lImp)
+      : RegsT * RuleLabelT
+      := match step with
+    | MkStep _ _ steps _ _  => Ts steps
+    end.
+
+  Hypothesis stateMapBeginsWell :
+    stateMap (initRegs (getRegInits imp)) = initRegs (getRegInits spec).
+
+  Hypothesis stateMapModular : forall (oImp u1 u2 uSpec1 uSpec2 : RegsT),
+    M.Disj u1 u2 -> M.Disj uSpec1 uSpec2
+  -> M.update (stateMap oImp) uSpec1 = stateMap (M.update oImp u1)
+  -> M.update (stateMap oImp) uSpec2 = stateMap (M.update oImp u2)
+  -> M.update (stateMap oImp) (M.union uSpec1 uSpec2) 
+  = stateMap (M.update oImp (M.union u1 u2)).
+
+  Hypothesis consistentSubstepMap : forall {oImp lImp nImp}
+   , (exists ruleLabel, Behavior imp oImp ruleLabel)
+   -> forall (step : UnitStep imp oImp nImp lImp)
+   , match T step with (nSpec, lSpec) =>
+      let oSpec := stateMap oImp in
+        (M.update oSpec nSpec = stateMap (M.update oImp nImp)
+      /\ equivalent lSpec lImp pRL)
+      * UnitStep spec oSpec nSpec lSpec
+     end.
+
+  Hypothesis specShouldCombine : forall {oImp} 
+  , (exists ruleLabel, Behavior imp oImp ruleLabel)
+  -> forall {nImp1 lImp1} (step1 : UnitStep imp oImp nImp1 lImp1)
+      {nImp2 lImp2} (step2 : UnitStep imp oImp nImp2 lImp2)
+  , CanCombine (nImp1, lImp1) (nImp2, lImp2)
+  -> CanCombine (T step1) (T step2).
+
+  Lemma pBeforeAfter : forall (l : RuleLabelT),
+    pMod id (mapLabelTP (fun _ : string => I) l) =
+     mapLabelTP (fun _ : string => I) (pRL l).
+  Proof. intros. unfold pRL, pMod.
+  destruct l. simpl.
+  destruct (p (dms0, cms0)). simpl.
+  destruct ruleMeth0; simpl; unfold id; reflexivity.
   Qed.
-End Domain.
 
-Section WellFormed.
-  Variable m1 m2: Modules.
-
-  Variable newRegsDomainM1: RegsInDomain m1.
-  Variable newRegsDomainM2: RegsInDomain m2.
-
-  Variable disjRegs:
-    forall r, ~ (In r (namesOf (getRegInits m1)) /\
-                 In r (namesOf (getRegInits m2))).
-  Variable r: RegsT.
-  Variable l: list RuleLabelT.
-
-  Theorem ltsStepClosure_split:
-    LtsStepClosure (ConcatMod m1 m2) r l ->
-    exists r1 r2 l1 l2,
-      LtsStepClosure m1 r1 l1 /\
-      LtsStepClosure m2 r2 l2 /\
-      MF.union r1 r2 = r /\
-      ConcatLabelSeq l1 l2 l.
-  Proof.
-    admit. (* Proof deprecated due to disjUnion -> union *)
-    (* intros clos. *)
-    (* remember (ConcatMod m1 m2) as m. *)
-    (* induction clos; rewrite Heqm in *; simpl in *. *)
-    (* - exists (initRegs (getRegInits m1)). *)
-    (*          exists (initRegs (getRegInits m2)). *)
-    (*          unfold initRegs, namesOf in *. *)
-    (*          rewrite (disjUnionProp (f1 := ConstFullT) (fullType type) evalConstFullT *)
-    (*                                 (getRegInits m1) (getRegInits m2)) in *. *)
-    (*          exists nil; exists nil. *)
-    (*          repeat (constructor || intuition). *)
-    (* - destruct (IHclos eq_refl) as [r1 [r2 [l1 [l2 [step1 [step2 [regs labels]]]]]]]; *)
-    (*   clear IHclos. *)
-    (*   inversion Hlts; subst. *)
-    (*   exists (update olds1 news1). *)
-    (*   exists (update olds2 news2). *)
-    (*   exists ((Build_RuleLabelT rm1 (getDmsMod m1) dmMap1 (getCmsMod m1) cmMap1) :: l1). *)
-    (*   exists ((Build_RuleLabelT rm2 (getDmsMod m2) dmMap2 (getCmsMod m2) cmMap2) :: l2). *)
-    (*   pose proof (regsDomain newRegsDomainM1 step1) as regs1. *)
-    (*   pose proof (regsDomain newRegsDomainM2 step2) as regs2. *)
-    (*   pose proof (disjUnion_div disjRegs regs1 regs2 HOldRegs1 HOldRegs2 Holds) as [H1 H2]. *)
-    (*   subst. *)
-    (*   constructor. *)
-    (*   + apply (lcLtsStep (or' := update olds1 news1) step1 Hlts1 eq_refl). *)
-    (*   + constructor. *)
-    (*     * apply (lcLtsStep (or' := update olds2 news2) step2 Hlts2 eq_refl). *)
-    (*     * constructor. *)
-    (*       { pose proof newRegsDomainM1 Hlts1 as H1. *)
-    (*         pose proof newRegsDomainM2 Hlts2 as H2. *)
-    (*         apply disjUnion_update_comm. *)
-    (*       } *)
-    (*       { constructor; intuition. } *)
+  Lemma canCombineLeft :
+    forall {t u1 u2 l1 l2},
+      CanCombine t (M.union u1 u2, mergeLabel l1 l2) ->
+      CanCombine t (u1, l1).
+  Proof. 
+    intros.
+    destruct l1 as [rm1 ds1 cs1].
+    destruct l2 as [rm2 ds2 cs2].
+    unfold CanCombine in H; dest; simpl in *.
+    constructor; try (eapply M.Disj_union_1; eassumption).
+    unfold NotBothRule in *.
+    destruct rm1.
+    - simpl; destruct H0; [|discriminate].
+      repeat split.
+      + left; auto.
+      + eapply M.Disj_union_1; eauto.
+      + eapply M.Disj_union_1; eauto.
+    - repeat split.
+      + right; auto.
+      + eapply M.Disj_union_1; eauto.
+      + eapply M.Disj_union_1; eauto.
   Qed.
-End WellFormed.
 
-(** Tactics for dealing with semantics *)
+  Lemma canCombineRight :
+    forall {t u1 u2 l1 l2},
+      CanCombine t (M.union u1 u2, mergeLabel l1 l2) ->
+      CanCombine t (u2, l2).
+  Proof.
+    intros.
+    destruct l1 as [rm1 ds1 cs1].
+    destruct l2 as [rm2 ds2 cs2].
+    unfold CanCombine in H; dest; simpl in *.
+    constructor; try (eapply M.Disj_union_2; eassumption).
+    unfold NotBothRule in *.
+    destruct rm1.
+    - simpl; destruct H0; [|discriminate].
+      repeat split.
+      + left; auto.
+      + eapply M.Disj_union_2; eauto.
+      + eapply M.Disj_union_2; eauto.
+    - simpl; destruct H0.
+      + repeat split.
+        * left; auto.
+        * eapply M.Disj_union_2; eauto.
+        * eapply M.Disj_union_2; eauto.
+      + repeat split.
+        * right; auto.
+        * eapply M.Disj_union_2; eauto.
+        * eapply M.Disj_union_2; eauto.
+  Qed.
 
-(*
-I got rid of this because I have no in_tac_ex
+  Lemma canCombineMerge : forall {t u1 u2 l1 l2},
+    CanCombine t (u1, l1)
+  -> CanCombine t (u2, l2)
+  -> CanCombine t (M.union u1 u2, mergeLabel l1 l2).
+  Proof.
+    admit.
+    (* intros. destruct t as [uL [rmL csL dsL]].  *)
+    (* destruct (mergeLabel l1 l2) as [rm1 cs ds] eqn:labeleqn. *)
+    (* inversion H; inversion H0; inversion labeleqn; subst. *)
+    (* econstructor. apply M.Disj_union; assumption. *)
+    (* apply M.Disj_union; assumption. *)
+    (* apply M.Disj_union; assumption. *)
+    (* unfold NotBothRule in *; destruct rmL, rm2, rm4; intuition. *)
+  Qed.  
 
-Ltac invStep :=
-  repeat
-    match goal with
-      | [Horig: LtsStep ?m None _ _ _ _ |- _] =>
-        let Ha := fresh "Ha" in
-        assert (Ha: exists lm rm, m = ConcatMod lm rm) by (repeat eexists);
-          clear Ha; inv Horig; destConcatLabel;
-          match goal with
-            | [Hcrm: CombineRm _ _ None |- _] =>
-              pose proof (combineRm_prop_5 Hcrm); dest; subst
-          end
-      | [Horig: LtsStep ?m (Some ?r) _ _ _ _ |- _] =>
-        let Ha := fresh "Ha" in
-        assert (Ha: exists lm rm, m = ConcatMod lm rm) by (repeat eexists);
-          clear Ha; inv Horig; destConcatLabel;
-          match goal with
-            | [Hcrm: CombineRm _ _ _, H: LtsStep ?m ?rm _ _ _ _ |- _] =>
-              let Hin := fresh "Hin" in
-              assert (Hin: ~ In r (namesOf (getRules m))) by in_tac_ex;
-                assert (rm = None) by
-                  (destruct rm; [exfalso; elim Hin|reflexivity];
-                   eapply ltsStep_rule; [eassumption|];
-                   (rewrite (combineRm_prop_1 Hcrm) || rewrite (combineRm_prop_2 Hcrm));
-                   reflexivity);
-                clear Hin; subst;
-                (rewrite (combineRm_prop_3 Hcrm) in * || rewrite (combineRm_prop_4 Hcrm) in * );
-                clear Hcrm
-          end
-    end;
-  repeat
-    match goal with
-      | [H: LtsStep ?m _ _ _ _ _ |- _] =>
-        let Ha := fresh "Ha" in
-        assert (Ha: exists m1 m2 m3, m = Mod m1 m2 m3) by (repeat eexists);
-          clear Ha; inv H
-    end.
-*)
+  Lemma canCombineSym : forall {t1 t2},
+    CanCombine t1 t2 -> CanCombine t2 t1.
+  Proof.
+    admit.
+   (* intros t1 t2 H; *)
+   (* inversion H; clear H; subst;  *)
+   (* constructor; eauto using M.Disj_comm. *)
+   (* unfold NotBothRule in *. *)
+   (* destruct rm1, rm2; intuition. *)
+  Qed. 
 
-Ltac destRule Hlts :=
-  match type of Hlts with
-    | (LtsStep _ ?rm _ _ _ _) =>
-      inv Hlts;
-        repeat match goal with
-                 | [H: SemMod _ _ rm _ _ _ _ |- _] =>
-                   destruct rm; [inv H; repeat match goal with
-                                                 | [H: In _ _ |- _] => inv H
-                                               end|]
-                 | [H: {| attrName := _; attrType := _ |} =
-                       {| attrName := _; attrType := _ |} |- _] => inv H
-               end
-  end.
+  Lemma specShouldCombines : forall {oImp} 
+  , (exists ruleLabel, Behavior imp oImp ruleLabel)
+  -> forall {nImp1 lImp1} (step1 : UnitSteps imp oImp nImp1 lImp1)
+      {nImp2 lImp2} (step2 : UnitSteps imp oImp nImp2 lImp2)
+  , CanCombine (nImp1, lImp1) (nImp2, lImp2)
+  -> CanCombine (Ts step1) (Ts step2).
+  Proof. 
+    intros oImp H nImp1 lImp1 US1. induction US1.
+    - intros nImp2 lImp2 US2. induction US2.
+      + apply specShouldCombine; assumption.
+      + intros.
+        simpl in IHUS2_1, IHUS2_2.
+        pose proof (IHUS2_1 (canCombineLeft H0)) as H21.
+        pose proof (IHUS2_2 (canCombineRight H0)) as H22.
+        simpl. destruct (Ts US2_1). destruct (Ts US2_2).
+        apply canCombineMerge; assumption.
+    - simpl in *. intros. apply canCombineSym.
+      destruct (Ts US1_1). destruct (Ts US1_2).
+      apply canCombineMerge; apply canCombineSym;
+      [apply IHUS1_1 | apply IHUS1_2]; try assumption;
+      apply canCombineSym in H0;
+      apply canCombineSym. 
+      eapply canCombineLeft; eassumption.
+      eapply canCombineRight; eassumption.    
+  Qed.
+  
+Require CommonTactics.
 
-Ltac destRuleRep :=
-  repeat match goal with
-           | [H: LtsStep _ _ _ _ _ _ |- _] => destRule H
-         end.
+  Lemma consistentUnitStepsMap : forall oImp lImp nImp
+    , (exists ruleLabel, Behavior imp oImp ruleLabel)
+      -> forall (steps : UnitSteps imp oImp nImp lImp)
+      , let (nSpec, lSpec) := Ts steps in
+        let oSpec := stateMap oImp in
+        (M.update oSpec nSpec = stateMap (M.update oImp nImp)
+         /\ equivalent lSpec lImp pRL)
+        * UnitSteps spec oSpec nSpec lSpec.
+  Proof.
+    admit.
+  (*   intros. *)
+  (*   induction steps; intros. *)
+  (*   - pose proof (consistentSubstepMap H u0). simpl in *. *)
+  (*     destruct (T u0) as [uSpec lSpec]. *)
+  (*     intuition. constructor. assumption. *)
+  (* - pose proof (specShouldCombines H steps1 steps2 c). *)
+  (*   simpl in *. *)
+  (*   destruct (Ts steps1) as [uSpec1 lSpec1]. *)
+  (*   destruct (Ts steps2) as [uSpec2 lSpec2]. *)
+  (*   intuition.  *)
+  (*   CommonTactics.inv c. CommonTactics.inv H0. *)
+  (*   apply stateMapModular; assumption. *)
+  (*   unfold equivalent in *. subst. *)
+  (*   CommonTactics.inv c. *)
+  (*   apply pmerge; assumption. *)
+  (*   apply UnitStepsUnion. assumption. assumption. *)
+  (*   unfold equivalent in *. *)
+  (*   assumption. *)
+  Qed.
+  
+  Lemma consistentStepMap : forall oImp lImp nImp
+    , (exists ruleLabel, Behavior imp oImp ruleLabel)
+      -> forall (step : Step imp oImp nImp lImp)
+      , let (nSpec, lSpec) := Ts' step in
+        let oSpec := stateMap oImp in
+        (M.update oSpec nSpec = stateMap (M.update oImp nImp))
+        * Step spec oSpec nSpec (pRL lImp).
+  Proof. 
+    intros.
+    destruct step eqn:stepeqn.
+    pose proof (consistentUnitStepsMap H u). simpl in *.
+    destruct (Ts u) as [nSpec lSpec]. 
+    intuition.  
+    econstructor. eassumption.
+    unfold equivalent in *. rewrite e.
+    rewrite H1. apply phide.
+    unfold equivalent in *. subst.
+    apply (pwellHidden _ w).
+  Qed. 
 
-Ltac combRule :=
-  match goal with
-    | [H: CombineRm (Some _) (Some _) _ |- _] =>
-      unfold CombineRm in H; destruct H as [[H|H] _]; inversion H
-    | [H: CombineRm None (Some _) _ |- _] =>
-      unfold CombineRm in H; destruct H as [_]; subst
-    | [H: CombineRm (Some _) None _ |- _] =>
-      unfold CombineRm in H; destruct H as [_]; subst
-    | [H: CombineRm None None _ |- _] =>
-      unfold CombineRm in H; destruct H as [_]; subst
-  end.
+  Theorem decomposition : TraceRefines imp spec (pMod id).
+  Proof.
+    unfold TraceRefines. intros.
+    exists (stateMap simp).
+    pose proof H.
+    inversion H0; clear H0; subst.
+    econstructor.
+    Focus 2. instantiate (1 := map pRL labels).
+    repeat rewrite map_map. apply map_ext.
+    intros. apply pBeforeAfter.
+    induction H1.
+    - rewrite <- stateMapBeginsWell. apply MSNil.
+    - assert (Behavior imp regs' (map (mapLabelTP (fun _ : string => I)) labels)).
+      econstructor. eassumption. reflexivity.
+      pose proof (consistentStepMap (ex_intro _ _ H2) X).
+      destruct (Ts' X) eqn:Ts'X.
+      destruct X0 as [HT1 HT2].
+      apply MSMulti with (regs' := stateMap regs') (u := r).
+      apply IHMultiStep. assumption.
+      assumption.
+      rewrite H0. rewrite <- HT1. reflexivity.
+  Qed.
 
-Ltac callIffDef_dest :=
-  repeat
-    match goal with
-      | [H: CallIffDef _ _ |- _] => unfold CallIffDef in H; dest
-    end;
-  unfold dmMap, cmMap, dms, cms in *.
-
-Ltac filt_dest :=
-  repeat
-    match goal with
-      | [H: FiltDm _ _ _ |- _] =>
-        unfold FiltDm in H;
-          unfold dmMap, cmMap, dms, cms in H;
-          subst
-      | [H: FiltCm _ _ _ |- _] =>
-        unfold FiltCm in H;
-          unfold dmMap, cmMap, dms, cms in H;
-          subst
-    end.
-
-Ltac basic_dest :=
-  repeat
-    match goal with
-      | [H: Some _ = Some _ |- _] => try (apply opt_some_eq in H; subst)
-      | [H: {| objType := _; objVal := _ |} = {| objType := _; objVal := _ |} |- _] =>
-        try (apply typed_eq in H; subst)
-      | [H: (_, _) = (_, _) |- _] => inv H; subst
-      | [H: existT _ _ _ = existT _ _ _ |- _] =>
-        try (apply Eqdep.EqdepTheory.inj_pair2 in H; subst)
-      | [H: Some _ = None |- _] => inversion H
-      | [H: None = Some _ |- _] => inversion H
-      | [H: true = false |- _] => inversion H
-      | [H: false = true |- _] => inversion H
-    end.
-
-(* same story: missing in_tac_ex
-Ltac pred_dest meth :=
-  repeat
-    match goal with
-      | [H: forall m: string, In m nil -> _ |- _] =>
-        clear H
-    end;
-  repeat
-    match goal with
-      | [H: forall m: string, In m _ -> _ |- _] =>
-        let Hin := type of (H meth) in
-        isNew Hin; let Hs := fresh "Hs" in pose proof (H meth) as Hs
-    end;
-  repeat
-    match goal with
-      | [H: In ?m ?l -> _ |- _] =>
-        (let Hp := fresh "Hp" in
-         assert (Hp: In m l)
-           by (repeat autounfold; repeat autounfold with ModuleDefs; in_tac_ex);
-         specialize (H Hp); clear Hp)
-          || (clear H)
-    end;
-  repeat
-    match goal with
-      | [H: find _ _ = _ |- _] => repeat autounfold in H; repeat (map_compute H)
-    end.
-*)
-
-(* missing map_simpl tactic
-Ltac invariant_tac :=
-  repeat
-    match goal with
-      | [H: find _ _ = Some _ |- _] => progress (map_simpl H)
-      | [H1: ?lh = Some _, H2: ?lh = Some _ |- _] =>
-        simpl in H1, H2; rewrite H1 in H2
-      | [H1: ?lh = Some _, H2: Some _ = ?lh |- _] =>
-        simpl in H1, H2; rewrite H1 in H2
-      | [H1: ?lh = true, H2: ?lh = false |- _] =>
-        simpl in H1, H2; rewrite H1 in H2
-      | [H1: ?lh = true, H2: false = ?lh |- _] =>
-        simpl in H1, H2; rewrite H1 in H2
-      | [H1: ?lh = false, H2: true = ?lh |- _] =>
-        simpl in H1, H2; rewrite H1 in H2
-      | [H1: if weq ?w1 ?w2 then _ else _, H2: ?w1 = ?w3 |- _] =>
-        rewrite H2 in H1; simpl in H1
-      | [H: ?w1 = ?w3 |- context [if weq ?w1 ?w2 then _ else _] ] =>
-        rewrite H; simpl
-    end.
-*)
-
-(* missing pred_dest tactic
-Ltac conn_tac meth :=
-  callIffDef_dest; filt_dest; pred_dest meth; repeat (invariant_tac; basic_dest).
-Ltac fconn_tac meth := exfalso; conn_tac meth.
-*)
-
-Ltac regsInDomain_tac := admit. (* TODO: reimplement *)
-  (* hnf; intros; *)
-  (* repeat match goal with *)
-  (*        | [ H : LtsStep _ _ _ _ _ _ |- _ ] => inv H *)
-  (*        | [ H : SemMod _ _ _ _ _ _ _ |- _ ] => inv H *)
-  (*        end; in_tac_H; (deattr; simpl in *; repeat invertActionRep; inDomain_tac). *)
-
-Global Opaque mkStruct.
+End Decomposition.
