examples/Fifo.v
@@ -77,12 +77,12 @@ Section Fifo.
     with Method ^"deq"() : dType := deq
   }.
 
-  Section Spec.
-    Lemma regsInDomain_simpleFifo: RegsInDomain simpleFifo.
-    Proof.
-      regsInDomain_tac.
-    Qed.
-  End Spec.
+  (* Section Spec. *)
+  (*   Lemma regsInDomain_simpleFifo: RegsInDomain simpleFifo. *)
+  (*   Proof. *)
+  (*     regsInDomain_tac. *)
+  (*   Qed. *)
+  (* End Spec. *)
 
 End Fifo.
 
