src/SemanticsExprAction.v
@@ -1,0 +1,411 @@
+Require Import Bool List String Structures.Equalities.
+Require Import Lib.Struct Lib.Word Lib.CommonTactics Lib.StringBound Lib.ilist Lib.FMap Syntax.
+Require Import FunctionalExtensionality Program.Equality Eqdep Eqdep_dec.
+
+Set Implicit Arguments.
+
+(* TODO: may move to lib/Struct.v *)
+Lemma opt_some_eq: forall {A} (v1 v2: A), Some v1 = Some v2 -> v1 = v2.
+Proof. intros; inv H; reflexivity. Qed.
+
+Lemma typed_type_eq:
+  forall {A} (a1 a2: A) (B: A -> Type) (v1: B a1) (v2: B a2),
+    {| objType := a1; objVal := v1 |} = {| objType := a2; objVal := v2 |} ->
+    exists (Heq: a1 = a2), match Heq with eq_refl => v1 end = v2.
+Proof. intros; inv H; exists eq_refl; reflexivity. Qed.
+
+Lemma typed_eq:
+  forall {A} (a: A) (B: A -> Type) (v1 v2: B a),
+    {| objType := a; objVal := v1 |} = {| objType := a; objVal := v2 |} ->
+    v1 = v2.
+Proof. intros; inv H; apply Eqdep.EqdepTheory.inj_pair2 in H1; assumption. Qed.
+
+(* concrete representations of data kinds *)
+Fixpoint type (t: Kind): Type :=
+  match t with
+    | Bool => bool
+    | Bit n => word n
+    | Vector nt n => word n -> type nt
+    | Struct attrs => forall i, @GetAttrType _ (map (mapAttr type) attrs) i
+  end.
+
+(*
+Fixpoint fullType (k : FullKind) : Type := match k with
+  | SyntaxKind t => type t
+  | NativeKind t => t
+  end.
+ *)
+
+Section WordFunc.
+
+  Definition wordZero (w: word 0): w = WO :=
+    shatter_word w.
+
+  Variable A: Type.
+
+  (* a lemma for wordVecDec *)
+  Definition wordVecDec':
+    forall n (f g: word n -> A), (forall x: word n, {f x = g x} + {f x <> g x}) ->
+                                 {forall x, f x = g x} + {exists x, f x <> g x}.
+  Proof.
+    intro n.
+    induction n; intros f g H.
+    - destruct (H WO).
+      + left; intros x.
+        rewrite (wordZero x) in *; intuition.
+      + right; eauto.
+    - assert (Hn: forall b (x: word n),
+                    {f (WS b x) = g (WS b x)} + {f (WS b x) <> g (WS b x)}) by
+             (intros; specialize (H (WS b x)); intuition).
+      destruct (IHn _ _ (Hn false)) as [ef | nf].
+      + destruct (IHn _ _ (Hn true)) as [et | nt].
+        * left; intros x.
+          specialize (ef (wtl x)).
+          specialize (et (wtl x)).
+          pose proof (shatter_word x) as use; simpl in *.
+          destruct (whd x); rewrite <- use in *; intuition.
+        * right; destruct_ex; eauto.
+      + right; destruct_ex; eauto.
+  Qed.
+
+  Definition wordVecDec:
+    forall n (f g: word n -> A), (forall x: word n, {f x = g x} + {f x <> g x}) ->
+                                 {f = g} + {f <> g}.
+  Proof.
+    intros.
+    pose proof (wordVecDec' _ _ H) as [lt | rt].
+    left; apply functional_extensionality; intuition.
+    right; unfold not; intros eq; rewrite eq in *.
+    destruct rt; intuition.
+  Qed.
+End WordFunc.
+
+Section VecFunc.
+  Variable A: Type.
+  Fixpoint evalVec n (vec: Vec A n): word n -> A.
+  Proof.
+    refine match vec in Vec _ n return word n -> A with
+             | Vec0 e => fun _ => e
+             | VecNext n' v1 v2 =>
+               fun w =>
+                 match w in word m0 return m0 = S n' -> A with
+                   | WO => _
+                   | WS b m w' =>
+                     if b
+                     then fun _ => evalVec _ v2 (_ w')
+                     else fun _ => evalVec _ v2 (_ w')
+                 end eq_refl
+           end;
+    clear evalVec.
+    abstract (intros; discriminate).
+    abstract (injection _H; intros; subst; intuition).
+    abstract (injection _H; intros; subst; intuition).
+  Defined.
+
+  Variable B: Type.
+  Variable map: A -> B.
+  Fixpoint mapVec n (vec: Vec A n): Vec B n :=
+    match vec in Vec _ n return Vec B n with
+      | Vec0 e => Vec0 (map e)
+      | VecNext n' v1 v2 => VecNext (mapVec v1) (mapVec v2)
+    end.
+End VecFunc.
+
+(* for any kind, we have decidable equality on its representation *)
+Definition isEq : forall k (e1: type k) (e2: type k),
+                    {e1 = e2} + {e1 <> e2}.
+Proof.
+  refine (fix isEq k : forall (e1: type k) (e2: type k), {e1 = e2} + {e1 <> e2} :=
+            match k return forall (e1: type k) (e2: type k),
+                             {e1 = e2} + {e1 <> e2} with
+              | Bool => bool_dec
+              | Bit n => fun e1 e2 => weq e1 e2
+              | Vector n nt =>
+                  fun e1 e2 =>
+                    wordVecDec e1 e2 (fun x => isEq _ (e1 x) (e2 x))
+              | Struct h =>
+                (fix isEqs atts : forall (vs1 vs2 : forall i, @GetAttrType _ (map (mapAttr type) atts) i),
+                                    {vs1 = vs2} + {vs1 <> vs2} :=
+                   match atts return forall (vs1 vs2 : forall i, @GetAttrType _ (map (mapAttr type) atts) i),
+                                       {vs1 = vs2} + {vs1 <> vs2} with
+                     | nil => fun _ _ => Yes
+                     | att :: atts' => fun vs1 vs2 =>
+                       isEq _
+                            (vs1 {| bindex := attrName att; indexb := {| ibound := 0;
+                                      boundi := eq_refl :
+                                                  nth_error
+                                                    (map (attrName (Kind:=Type))
+                                                         (map (mapAttr type) (att :: atts'))) 0
+                                                    = Some (attrName att) |} |})
+                            (vs2 {| bindex := attrName att; indexb := {| ibound := 0;
+                                      boundi := eq_refl :
+                                                  nth_error
+                                                    (map (attrName (Kind:=Type))
+                                                         (map (mapAttr type) (att :: atts'))) 0
+                                                    = Some (attrName att) |} |});;
+                       isEqs atts'
+                       (fun i => vs1 {| indexb := {| ibound := S (ibound (indexb i)) |} |})
+                       (fun i => vs2 {| indexb := {| ibound := S (ibound (indexb i)) |} |});;
+                       Yes
+                   end) h
+            end); clear isEq; try clear isEqs;
+  abstract (unfold BoundedIndexFull in *; simpl in *; try (intro; subst; tauto);
+  repeat match goal with
+           | [ |- _ = _ ] => extensionality i
+           | [ x : BoundedIndex _ |- _ ] => destruct x
+           | [ x : IndexBound _ _ |- _ ] => destruct x
+           | [ H : nth_error nil ?n = Some _ |- _ ] => destruct n; discriminate
+           | [ |- _ {| indexb := {| ibound := ?b |} |} = _ ] =>
+             match goal with
+               | [ x : _ |- _ ] =>
+                 match x with
+                   | b => destruct b; simpl in *
+                 end
+             end
+           | [ H : Specif.value _ = Some _ |- _ ] => progress (injection H; intro; subst)
+           | [ H : _ = _ |- _ ] => progress rewrite (UIP_refl _ _ H)
+           | [ H : _ = _ |- _ {| bindex := ?bi; indexb := {| ibound := S ?ib; boundi := ?pf |} |} = _ ] =>
+             apply (f_equal (fun f => f {| bindex := bi; indexb := {| ibound := ib; boundi := pf |} |})) in H
+         end; auto).
+Defined.
+
+Definition evalUniBool (op: UniBoolOp) : bool -> bool :=
+  match op with
+    | Neg => negb
+  end.
+
+Definition evalBinBool (op: BinBoolOp) : bool -> bool -> bool :=
+  match op with
+    | And => andb
+    | Or => orb
+  end.
+
+(* the head of a word, or false if the word has 0 bits *)
+Definition whd' sz (w: word sz) :=
+  match sz as s return word s -> bool with
+    | 0 => fun _ => false
+    | S n => fun w => whd w
+  end w.
+
+Definition evalUniBit n1 n2 (op: UniBitOp n1 n2): word n1 -> word n2.
+refine match op with
+         | Inv n => @wneg n
+         | ConstExtract n1 n2 n3 => fun w => split2 n1 n2 (split1 (n1 + n2) n3 w)
+         | ZeroExtendTrunc n1 n2 => fun w => split2 n1 n2 (_ (combine (wzero n2) w))
+         | SignExtendTrunc n1 n2 => fun w => split2 n1 n2 (_ (combine (if whd' w
+                                                                       then wones n2
+                                                                       else wzero n2) w))
+         | TruncLsb n1 n2 => fun w => split1 n1 n2 w
+       end;
+  assert (H: n3 + n0 = n0 + n3) by omega;
+  rewrite H in *; intuition.
+Defined.
+
+Definition evalBinBit n1 n2 n3 (op: BinBitOp n1 n2 n3)
+  : word n1 -> word n2 -> word n3 :=
+  match op with
+    | Add n => @wplus n
+    | Sub n => @wminus n
+  end.
+
+Definition evalConstStruct attrs (ils : ilist (fun a => type (attrType a)) attrs) : type (Struct attrs) :=
+  fun (i: BoundedIndex (namesOf (map (mapAttr type) attrs))) =>
+    mapAttrEq1 type attrs i
+               (ith_Bounded _ ils (getNewIdx1 type attrs i)).
+
+(* evaluate any constant operation *)
+Fixpoint evalConstT k (e: ConstT k): type k :=
+  match e in ConstT k return type k with
+    | ConstBool b => b
+    | ConstBit n w => w
+    | ConstVector k' n v => evalVec (mapVec (@evalConstT k') v)
+    | ConstStruct attrs ils => evalConstStruct (imap _ (fun _ ba => evalConstT ba) ils)
+  end.
+
+Definition evalConstFullT k (e: ConstFullT k) :=
+  match e in ConstFullT k return fullType type k with
+    | SyntaxConst k' c' => evalConstT c'
+    | NativeConst t c c' => c'
+  end.
+
+(* maps register names to the values which they currently hold *)
+Definition RegsT := M.t (Typed (fullType type)).
+
+(* a pair of the value sent to a method call and the value it returned *)
+Definition SignT k := (type (arg k) * type (ret k))%type.
+
+(* a list of simulatenous method call actions made during a single step *)
+Definition CallsT := M.t (Typed SignT).
+
+Section Semantics.
+  Definition mkStruct attrs (ils : ilist (fun a => type (attrType a)) attrs) : type (Struct attrs) :=
+    fun (i: BoundedIndex (namesOf (map (mapAttr type) attrs))) =>
+      mapAttrEq1 type attrs i (ith_Bounded _ ils (getNewIdx1 type attrs i)).
+
+  Fixpoint evalExpr exprT (e: Expr type exprT): fullType type exprT :=
+    match e in Expr _ exprT return fullType type exprT with
+      | Var _ v => v
+      | Const _ v => evalConstT v
+      | UniBool op e1 => (evalUniBool op) (evalExpr e1)
+      | BinBool op e1 e2 => (evalBinBool op) (evalExpr e1) (evalExpr e2)
+      | UniBit n1 n2 op e1 => (evalUniBit op) (evalExpr e1)
+      | BinBit n1 n2 n3 op e1 e2 => (evalBinBit op) (evalExpr e1) (evalExpr e2)
+      | ITE _ p e1 e2 => if evalExpr p
+                         then evalExpr e1
+                         else evalExpr e2
+      | Eq _ e1 e2 => if isEq _ (evalExpr e1) (evalExpr e2)
+                      then true
+                      else false
+      | ReadIndex _ _ i f => (evalExpr f) (evalExpr i)
+      | ReadField heading fld val =>
+          mapAttrEq2 type fld
+            ((evalExpr val) (getNewIdx2 type fld))
+      | BuildVector _ k vec => evalVec (mapVec (@evalExpr _) vec)
+      | BuildStruct attrs ils => mkStruct (imap _ (fun _ ba => evalExpr ba) ils)
+      | UpdateVector _ _ fn i v =>
+          fun w => if weq w (evalExpr i) then evalExpr v else (evalExpr fn) w
+    end.
+
+  (*register names and constant expressions for their initial values *)
+  Variable regInit: list RegInitT.
+
+  Variable rules: list (Attribute (Action (Bit 0))).
+
+  (* register values just before the current cycle *)
+  Variable oldRegs: RegsT.
+
+  Inductive SemAction:
+    forall k, ActionT type k -> RegsT -> CallsT -> type k -> Prop :=
+  | SemMCall
+      meth s (marg: Expr type (SyntaxKind (arg s)))
+      (mret: type (ret s))
+      retK (fret: type retK)
+      (cont: type (ret s) -> ActionT type retK)
+      newRegs (calls: CallsT) acalls
+      (HAcalls: acalls = M.add meth {| objVal := (evalExpr marg, mret) |} calls)
+      (HSemAction: SemAction (cont mret) newRegs calls fret):
+      SemAction (MCall meth s marg cont) newRegs acalls fret
+  | SemLet
+      k (e: Expr type k) retK (fret: type retK)
+      (cont: fullType type k -> ActionT type retK) newRegs calls
+      (HSemAction: SemAction (cont (evalExpr e)) newRegs calls fret):
+      SemAction (Let_ e cont) newRegs calls fret
+  | SemReadReg
+      (r: string) regT (regV: fullType type regT)
+      retK (fret: type retK) (cont: fullType type regT -> ActionT type retK)
+      newRegs calls
+      (HRegVal: M.find r oldRegs = Some {| objType := regT; objVal := regV |})
+      (HSemAction: SemAction (cont regV) newRegs calls fret):
+      SemAction (ReadReg r _ cont) newRegs calls fret
+  | SemWriteReg
+      (r: string) k
+      (e: Expr type k)
+      retK (fret: type retK)
+      (cont: ActionT type retK) newRegs calls anewRegs
+      (HANewRegs: anewRegs = M.add r {| objVal := (evalExpr e) |} newRegs)
+      (HSemAction: SemAction cont newRegs calls fret):
+      SemAction (WriteReg r e cont) anewRegs calls fret
+  | SemIfElseTrue
+      (p: Expr type (SyntaxKind Bool)) k1
+      (a: ActionT type k1)
+      (a': ActionT type k1)
+      (r1: type k1)
+      k2 (cont: type k1 -> ActionT type k2)
+      newRegs1 newRegs2 calls1 calls2 (r2: type k2)
+      (HTrue: evalExpr p = true)
+      (HAction: SemAction a newRegs1 calls1 r1)
+      (HSemAction: SemAction (cont r1) newRegs2 calls2 r2)
+      unewRegs ucalls
+      (HUNewRegs: unewRegs = M.union newRegs1 newRegs2)
+      (HUCalls: ucalls = M.union calls1 calls2):
+      SemAction (IfElse p a a' cont) unewRegs ucalls r2
+  | SemIfElseFalse
+      (p: Expr type (SyntaxKind Bool)) k1
+      (a: ActionT type k1)
+      (a': ActionT type k1)
+      (r1: type k1)
+      k2 (cont: type k1 -> ActionT type k2)
+      newRegs1 newRegs2 calls1 calls2 (r2: type k2)
+      (HFalse: evalExpr p = false)
+      (HAction: SemAction a' newRegs1 calls1 r1)
+      (HSemAction: SemAction (cont r1) newRegs2 calls2 r2)
+      unewRegs ucalls
+      (HUNewRegs: unewRegs = M.union newRegs1 newRegs2)
+      (HUCalls: ucalls = M.union calls1 calls2):
+      SemAction (IfElse p a a' cont) unewRegs ucalls r2
+  | SemAssertTrue
+      (p: Expr type (SyntaxKind Bool)) k2
+      (cont: ActionT type k2) newRegs2 calls2 (r2: type k2)
+      (HTrue: evalExpr p = true)
+      (HSemAction: SemAction cont newRegs2 calls2 r2):
+      SemAction (Assert_ p cont) newRegs2 calls2 r2
+  | SemReturn
+      k (e: Expr type (SyntaxKind k)) evale
+      (HEvalE: evale = evalExpr e):
+      SemAction (Return e) (M.empty _) (M.empty _) evale.
+
+  Theorem inversionSemAction
+          k a news calls retC
+          (evalA: @SemAction k a news calls retC):
+    match a with
+      | MCall m s e c =>
+        exists mret pcalls,
+          SemAction (c mret) news pcalls retC /\
+          calls = M.add m {| objVal := (evalExpr e, mret) |} pcalls
+      | Let_ _ e cont =>
+        SemAction (cont (evalExpr e)) news calls retC
+      | ReadReg r k c =>
+        exists rv,
+          M.find r oldRegs = Some {| objType := k; objVal := rv |} /\
+          SemAction (c rv) news calls retC
+      | WriteReg r _ e a =>
+        exists pnews,
+          SemAction a pnews calls retC /\
+          news = M.add r {| objVal := evalExpr e |} pnews
+      | IfElse p _ aT aF c =>
+        exists news1 calls1 news2 calls2 r1,
+          match evalExpr p with
+            | true =>
+              SemAction aT news1 calls1 r1 /\
+              SemAction (c r1) news2 calls2 retC /\
+              news = M.union news1 news2 /\
+              calls = M.union calls1 calls2
+            | false =>
+              SemAction aF news1 calls1 r1 /\
+              SemAction (c r1) news2 calls2 retC /\
+              news = M.union news1 news2 /\
+              calls = M.union calls1 calls2
+          end
+      | Assert_ e c =>
+        SemAction c news calls retC /\
+        evalExpr e = true
+      | Return e =>
+        retC = evalExpr e /\
+        news = M.empty _ /\
+        calls = M.empty _
+    end.
+  Proof.
+    destruct evalA; eauto; repeat eexists; destruct (evalExpr p); eauto; try discriminate.
+  Qed.
+End Semantics.
+
+Ltac invertAction H := apply inversionSemAction in H; simpl in H; dest; try subst.
+Ltac invertActionFirst :=
+  match goal with
+    | [H: SemAction _ _ _ _ _ |- _] => invertAction H
+  end.
+Ltac invertActionRep :=
+  repeat
+    match goal with
+      | [H: SemAction _ _ _ _ _ |- _] => invertAction H
+      | [H: if ?c
+            then
+              SemAction _ _ _ _ _ /\ _ /\ _ /\ _
+            else
+              SemAction _ _ _ _ _ /\ _ /\ _ /\ _ |- _] =>
+        let ic := fresh "ic" in
+        (remember c as ic; destruct ic; dest; subst)
+    end.
+
+Global Opaque mkStruct.
+
